implement init and partially implement serviceExchangeSymbols

bce/service.dfy
@@ -3,21 +3,114 @@ include "node.dfy"
 module BCE_Protocol_Service {
 import opened BCE_Protocol_Node
 
+datatype ServiceState = SPhase1 | SPhase2 | SDecided
 
-datatype ServiceState = ServiceState(
-    nodes:set<Node>
+datatype Service = Service(
+    nodes: seq<Node>,
+    n: nat,
+    f: nat,
+    state: ServiceState
 )
 
-predicate Service_Init(s: ServiceState)
+
+/****************************************************************************************/
+/*                                  PROTOCOL STEPS                                      */
+/****************************************************************************************/   
+
+
+predicate serviceInit(s: Service)
+{
+    && s.f > 0
+    && s.n == 3*s.f + 1
+    && |s.nodes| == s.n
+    && forall id :: 0 <= id < |s.nodes| ==> nodeInit(s.nodes[id], s.f, s.n, id)
+    && s.state == SPhase1
+}
+
+predicate serviceExchangeSymbols(s: Service, s': Service) 
+    requires serviceInit(s)
+{
+    var symbolsForExchange := symbolsToExchange(s.nodes);
+    lemma_Exchange_Generates_One_SymbolSeq_For_Each_Node(s.nodes);
+    lemma_Extract_Generates_One_Symbol_For_Each_Node(s.nodes);
+    lemma_Exchanged_Symbols_Are_Extracted(s.nodes, symbolsForExchange, 0);
+    assert |symbolsForExchange| == |s.nodes|;
+    && s' == s.(nodes := s'.nodes)
+    && |s'.nodes| == |s.nodes|
+    && forall id :: 0 <= id < |s.nodes| ==> 
+        assert symbolsForExchange[id][id] == s.nodes[id].codeword[id];
+        nodeReceiveSymbols(s.nodes[id], s'.nodes[id], symbolsForExchange[id])
+}
+
+
+predicate serviceNext(s:Service, s':Service)
 {
     // TODO
     true
 }
 
-predicate Service_Next(s:ServiceState, s':ServiceState)
+
+/****************************************************************************************/
+/*                             FUNCTIONS & PREDICATES                                   */
+/****************************************************************************************/ 
+
+
+/* Helper function for SPhase1 -> SPhase2 transition. 
+* symbolsToExchange(nodes)[i] represents the seq of symbols that nodes[i] receives in 
+* the exhange phase */
+function symbolsToExchange(nodes: seq<Node>) : seq<seq<symbol>> 
+    decreases nodes;
+    requires forall s :: s in nodes ==> s.n == 3*s.f + 1;
+    requires forall s :: s in nodes ==> 0 <= s.id < s.n;
+    requires forall s :: s in nodes ==> nodeInit(s, s.f, s.n, s.id)
 {
-    // TODO
-    true
+    if |nodes| == 0 then [] else
+    [extractSymbols(nodes)] + symbolsToExchange(nodes[1..])
+}
+
+/* Helper function that generates a single seq<symbol> for exchange. 
+* This is where Byzantine behavior can be modeled */
+function extractSymbols(nodes: seq<Node>) : seq<symbol> 
+    decreases nodes;
+    requires forall s :: s in nodes ==> s.n == 3*s.f + 1;
+    requires forall s :: s in nodes ==> 0 <= s.id < s.n;
+    requires forall s :: s in nodes ==> nodeInit(s, s.f, s.n, s.id)
+{
+    if |nodes| == 0 then [] else
+    [nodes[0].codeword[nodes[0].id]] + extractSymbols(nodes[1..])
+}
+
+
+/****************************************************************************************/
+/*                                       LEMMAS                                         */
+/****************************************************************************************/ 
+
+
+/* Proof that for any nodes: seq<Node>, |symbolsToExchange(nodes)| == |nodes| */
+lemma {:induction nodes} lemma_Exchange_Generates_One_SymbolSeq_For_Each_Node(nodes: seq<Node>) 
+    requires forall s :: s in nodes ==> s.n == 3*s.f + 1;
+    requires forall s :: s in nodes ==> 0 <= s.id < s.n;
+    requires forall s :: s in nodes ==> nodeInit(s, s.f, s.n, s.id)
+    ensures |symbolsToExchange(nodes)| == |nodes|;
+{}
+
+
+/* Proof that for any nodes: seq<Node>, |extractSymbols(nodes)| == |nodes| */
+lemma {:induction nodes} lemma_Extract_Generates_One_Symbol_For_Each_Node(nodes: seq<Node>) 
+    requires forall s :: s in nodes ==> s.n == 3*s.f + 1;
+    requires forall s :: s in nodes ==> 0 <= s.id < s.n;
+    requires forall s :: s in nodes ==> nodeInit(s, s.f, s.n, s.id)
+    ensures |extractSymbols(nodes)| == |nodes|;
+{}
+
+
+lemma  {:induction nodes} lemma_Exchanged_Symbols_Are_Extracted(nodes: seq<Node>, symbolsForExchange: seq<seq<symbol>>, i: nat) 
+    requires forall s :: s in nodes ==> s.n == 3*s.f + 1;
+    requires forall s :: s in nodes ==> 0 <= s.id < s.n;
+    requires forall s :: s in nodes ==> nodeInit(s, s.f, s.n, s.id)
+    ensures forall id :: 0 <= id < |symbolsForExchange| ==> symbolsForExchange[id] == extractSymbols(nodes);
+{
+    //TODO
 }
 
 
